cava/arrow-examples/SyntaxExamples.v
@@ -1,33 +1,28 @@
-Require Import Coq.Program.Tactics.
-Require Import Coq.Bool.Bool.
-Require Import Coq.Lists.List.
-Require Import Coq.Strings.String.
-Require Import Coq.Lists.Streams.
-
-Import ListNotations.
-
-From Coq Require Import ZArith.
-From Coq Require Import btauto.Btauto.
-
-Require Import Cava.Netlist.
-
 Require Import Cava.Arrow.Arrow.
 Require Import Cava.Arrow.Kappa.Syntax.
 Require Import Cava.Arrow.Instances.Combinational.
-Require Import Cava.Arrow.Instances.Netlist.
 
-Open Scope source.
+Require Import Coq.Strings.String.
+Local Open Scope string_scope.
 
-Definition xilinxFullAdder
-  : Kappa (bit ** (bit ** bit) ** unit) (bit**bit) :=
-  <[ \ cin ab =>
-     let a = fst' ab in
-     let b = snd' ab in
-     let part_sum = !xor_gate a b in
-     let sum      = !xorcy part_sum cin in
-     let cout     = !muxcy part_sum (cin, a) in
-     (sum, cout)
-  ]>.
+From Coq Require Import Lists.List.
+Import ListNotations.
 
-Definition xilinxFullAdder' := Closure_conversion xilinxFullAdder.
+Section definition.
+  Import KappaNotation. 
 
+  Definition xilinxFullAdder
+    : Kappa_sugared << Bit, << Bit, Bit >>, Unit >> << Bit, Bit >> :=
+    <[ \ cin ab =>
+      let '(a,b) = ab in
+      let part_sum = xor a b in
+      let sum      = xorcy part_sum cin in
+      let cout     = muxcy part_sum (cin, a) in
+      (sum, cout)
+    ]>.
+
+  Definition xilinxFullAdder_structure := (ltac: (build_structure xilinxFullAdder)).
+End definition.
+
+Lemma xilinxFullAdder_is_combinational: wf_combinational (toCava _ xilinxFullAdder_structure).
+Proof. combinational_obvious. Qed.
