cava/cava/Cava/Arrow/Kappa/CC.v
@@ -38,7 +38,6 @@ Hint Extern 2 => solver : core.
 
 Hint Extern 4 (_ < length (_ :: _)) => simpl : core.
 
-
 Notation "f ~ p" := 
   (eq_rect _ (fun x : Set => x) f _ p) (at level 70).
 
@@ -49,469 +48,469 @@ Notation "f ~ p" :=
   intros; congruence.
 Qed.
 
+(****************************************************************************)
+(* Environment manipulation                                                 *)
+(****************************************************************************)
 
-  (****************************************************************************)
-  (* Environment manipulation                                                 *)
-  (****************************************************************************)
+(* An environment to track the arrow Kinds corresponding to variables.
+Variables are then instantiated as a morphism from the environment to the
+associated Kind. *)
+Inductive environment : nat -> Type :=
+| ECons : forall n, Kind -> environment n -> environment (S n)
+| ENil : environment 0.
 
-  (* An environment to track the arrow objects corresponding to variables.
-  Variables are then instantiated as a morphism from the environment to the
-  associated object. *)
-  Inductive environment : nat -> Type :=
-  | ECons : forall n, bundle -> environment n -> environment (S n)
-  | ENil : environment 0.
+Fixpoint as_kind {n} (env: environment n): Kind :=
+match env with
+| ENil => Unit
+| ECons o env' => Tuple o (as_kind env')
+end.
 
-  Fixpoint as_object {n} (env: environment n): bundle :=
-  match env with
-  | ENil => Empty
-  | ECons o env' => Tuple2 o (as_object env')
-  end.
+Fixpoint as_kind_list {n} (env: environment n): list (Kind) :=
+match env with
+| ENil => []
+| ECons o env' => o :: as_kind_list env'
+end.
 
-  Fixpoint as_object_list {n} (env: environment n): list (bundle) :=
-  match env with
-  | ENil => []
-  | ECons o env' => o :: as_object_list env'
-  end.
+Fixpoint lookup_kind (n: nat) (env: list (Kind)): option (Kind) :=
+match env with
+| [] => None
+| o :: os =>
+  if eq_nat_dec n (length os)
+  then Some o
+  else lookup_kind n os
+end.
 
-  Fixpoint lookup_object (n: nat) (env: list (bundle)): option (bundle) :=
-  match env with
-  | [] => None
-  | o :: os =>
-    if eq_nat_dec n (length os)
+(* The type of an arrow morphism from our environment to a variable is
+`as_kind env ~> o`
+where lookup_kind n env = Some o *)
+Fixpoint lookup_morphism_ty (n: nat) (env_obj: Kind) (objs: list (Kind)): Type :=
+match objs with
+| [] => Datatypes.unit
+| o::os =>
+  if eq_nat_dec n (length os)
+  then structure env_obj o
+  else lookup_morphism_ty n env_obj os
+end.
+
+Fixpoint list_as_kind (l: list (Kind)): (Kind) :=
+match l with
+| [] => Unit
+| o :: os => Tuple o (list_as_kind os)
+end.
+
+(****************************************************************************)
+(* Environment lemmas                                                       *)
+(****************************************************************************)
+
+Lemma as_kind_is_as_list_as_kind: 
+  forall n (env: environment n), list_as_kind (as_kind_list env) = as_kind env.
+Proof.
+  intros.
+  induction env.
+  simpl.
+  f_equal.
+  apply IHenv.
+  simpl.
+  reflexivity.
+Defined.
+
+Definition Kind_to_list_kind_id: forall n (env: environment n), structure (as_kind env) (list_as_kind (as_kind_list env)).
+Proof.
+  intros.
+  rewrite as_kind_is_as_list_as_kind.
+  exact Id.
+Defined.
+
+Lemma lookup_bound:
+  forall n o objs,
+  lookup_kind n objs = Some o
+  -> n < length objs.
+Proof.
+  induction objs; auto.
+Qed.
+
+Hint Extern 3 =>
+  match goal with
+  | [H: lookup_kind _ _ = Some _|- _] => apply lookup_bound in H as H1
+  end : core.
+
+Lemma lookup_lower_contra : forall o n,
+  lookup_kind n [] = Some o -> False.
+Proof.
+  auto.
+Qed.
+
+Lemma lookup_upper_contra : forall o objs,
+  lookup_kind (length objs) objs = Some o -> False.
+Proof.
+  auto.
+Qed.
+
+Hint Extern 1 =>
+  match goal with
+  | [H: lookup_kind (length ?X) (?X) = Some _ |- _] => apply lookup_upper_contra in H; contradiction
+  | [H: lookup_kind ?X [] = Some _ |- _] => apply lookup_lower_contra in H; contradiction
+  end : core.
+
+(* Shorthand for passing evidence that a lookup is well formed *)
+Notation ok_lookup := (
+  fun (n: nat) (env: list (Kind)) (o: Kind) => lookup_kind n env = Some o
+).
+
+(* Proof that looking up a morphism is the morphism from the environment to
+  * the Kind at the same index.
+  *)
+Lemma ok_lookup_sets_lookup_morphism_ty : forall n o objs env_obj,
+  lookup_kind n objs = Some o
+  -> lookup_morphism_ty n env_obj objs = structure env_obj o.
+Proof.
+  induction objs; auto.
+Qed.
+
+Hint Immediate ok_lookup_sets_lookup_morphism_ty : core.
+
+Lemma morphism_coerce:
+  forall (n:nat) env_obj o (objs: list (Kind)),
+  ok_lookup n objs o ->
+  lookup_morphism_ty n env_obj objs = structure env_obj o.
+Proof.
+  auto.
+Qed.
+
+Lemma environment_kinds_length_is_n  (n: nat) (env: environment n):
+  length (as_kind_list env) = n.
+Proof.
+  induction env; auto.
+Qed.
+
+Hint Extern 4 =>
+  match goal with
+  | [H: context[length(as_kind_list ?X)] |- _] => rewrite environment_kinds_length_is_n in H
+  end : core.
+
+Lemma split_lookup : forall n env v1 y o,
+  ((n = v1 /\ y = o) \/ lookup_kind v1 (as_kind_list env) = Some o)
+  -> lookup_kind v1 (as_kind_list (@ECons n y env)) = Some o.
+Proof.
+  auto 6.
+Qed.
+
+Lemma unsplit_lookup : forall n env v1 y o,
+  lookup_kind v1 (as_kind_list (@ECons n y env)) = Some o
+  ->
+  ((n = v1 /\ y = o) \/ lookup_kind v1 (as_kind_list env) = Some o).
+Proof.
+  auto 6.
+Qed.
+
+Lemma lookup_top_is_top_kind: forall n m o o' env,
+  m = n
+  -> lookup_kind m (as_kind_list (@ECons n o env)) = Some o'
+  -> o = o'.
+Proof.
+  auto.
+Qed.
+
+Lemma push_lookup : forall n env o o' x ,
+  x <> n ->
+  lookup_kind x (as_kind_list (@ECons n o' env)) = Some o ->
+  lookup_kind x (as_kind_list env) = Some o.
+Proof.
+  Hint Extern 1 => lia : core.
+  auto.
+Qed.
+
+Fixpoint extract_nth n (env: environment n) o x
+  : (lookup_kind x (as_kind_list env) = Some o) -> structure (as_kind env) o :=
+match env return
+  (lookup_kind x (as_kind_list env) = Some o) -> structure (as_kind env) o
+  with
+| ENil => fun H => match lookup_lower_contra H with end
+| @ECons n' o' env' => fun H =>
+  match eq_nat_dec x n' with
+  | left Heq =>
+    match lookup_top_is_top_kind _ _ Heq H with
+    | eq_refl => Second Drop >>> Cancelr
+    end
+  | right Hneq => First Drop >>> Cancell >>> extract_nth env' x (push_lookup _ _ Hneq H)
+  end
+end.
+
+Notation "i ?? x" := (
+    match x with
+    | None => Datatypes.unit
+    | Some o => structure i o
+    end) (no associativity, at level 70).
+
+Fixpoint extract_nth' (env: list (Kind)) x : forall i (prefix: structure i (list_as_kind env)), i ?? lookup_kind x env :=
+match env return
+  forall i (prefix: structure i (list_as_kind env)), i ?? lookup_kind x env
+  with
+| [] => fun _ _ => tt
+| o :: os => 
+  match eq_nat_dec x (length os) as Heq return forall i (prefix: structure i (list_as_kind (o::os))), i ?? (if Heq
     then Some o
-    else lookup_object n os
-  end.
+    else lookup_kind x os
+  ) 
+  with
+  | left Heq => fun _ p => p >>> Second Drop >>> Cancelr
+  | right Hneq => fun _ p => extract_nth' os x (p >>> First Drop >>> Cancell)
+  end
+end.
 
-  (* The type of an arrow morphism from our environment to a variable is
-  `as_object env ~> o`
-  where lookup_object n env = Some o *)
-  Fixpoint lookup_morphism_ty (n: nat) (env_obj: bundle) (objs: list (bundle)): Type :=
-  match objs with
-  | [] => Datatypes.unit
-  | o::os =>
-    if eq_nat_dec n (length os)
-    then structure env_obj o
-    else lookup_morphism_ty n env_obj os
-  end.
+Lemma extractable : forall n env o,
+  lookup_kind n env = Some o
+  -> forall i (prefix: structure i (list_as_kind env)), i ?? lookup_kind n env = structure i o.
+Proof.
+  intros.
+  rewrite H.
+  reflexivity.
+Defined.
 
-  Fixpoint list_as_object (l: list (bundle)): (bundle) :=
-  match l with
-  | [] => Empty
-  | o :: os => Tuple2 o (list_as_object os)
-  end.
+(****************************************************************************)
+(* Closure conversion via de Brujin indices form                            *)
+(****************************************************************************)
+(* In de Brujin indexing variables are nats *)
 
-  (****************************************************************************)
-  (* Environment lemmas                                                       *)
-  (****************************************************************************)
+Definition natvar `{Category} : Kind -> Kind -> Type := fun _ _ => nat.
 
-  Lemma as_object_is_as_list_as_object: 
-    forall n (env: environment n), list_as_object (as_object_list env) = as_object env.
-  Proof.
-    intros.
-    induction env.
-    simpl.
-    f_equal.
-    apply IHenv.
-    simpl.
-    reflexivity.
-  Defined.
+(* Reverse de Brujin indexing is well formed *)
+Fixpoint wf_debrujin {i o}
+  (n: nat) (env: environment n)
+  (expr: @kappa natvar i o) {struct expr}
+  : Prop :=
+match expr with
+| DVar x            => ok_lookup x (as_kind_list env) o
+| @DAbs _ x y z f => wf_debrujin (@ECons n x env) (f n)
+| DApp e1 e2        => wf_debrujin env e1 /\ wf_debrujin env e2
+| DCompose e1 e2    => wf_debrujin env e1 /\ wf_debrujin env e2
+| DArr _            => True
+end.
 
-  Definition object_to_list_object_id: forall n (env: environment n), structure (as_object env) (list_as_object (as_object_list env)).
-  Proof.
-    intros.
-    rewrite as_object_is_as_list_as_object.
-    exact Id.
-  Defined.
+Lemma wf_debrujin_succ:
+  forall ix iy o
+  (n: nat) (env: environment n)
+  (expr: @kappa natvar (Tuple ix iy) o)
+  f,
+  expr = DAbs f ->
+  @wf_debrujin (Tuple ix iy) o n env expr -> @wf_debrujin iy o (S n) (ECons ix env) (f n).
+Proof.
+  auto.
+Defined.
 
-  Lemma lookup_bound:
-    forall n o objs,
-    lookup_object n objs = Some o
-    -> n < length objs.
-  Proof.
-    induction objs; auto.
-  Qed.
 
-  Hint Extern 3 =>
-    match goal with
-    | [H: lookup_object _ _ = Some _|- _] => apply lookup_bound in H as H1
-    end : core.
+(* Perform closure conversion by passing an explicit environment. The higher
+order PHOAS representation is converted to first order form with de Brujin
+indexing as described by Adam Chlipala's Lambda Tamer project. As our source
+language is a Kappa calculus and our target is a Generalized Arrow representation,
+the environment and arguments are manipulated using Arrow combinators amongst
+other differences.
 
-  Lemma lookup_lower_contra : forall o n,
-    lookup_object n [] = Some o -> False.
-  Proof.
-    auto.
-  Qed.
+This implementation is also currently missing logic to remove free variables
+from the environment.
+*)
+Fixpoint closure_conversion' {i o}
+  (n: nat) (env: environment n)
+  (* (morphs: env_morphisms (as_kind env) (as_kind_list env)) *)
+  (expr: @kappa natvar i o) {struct expr}
+  : wf_debrujin env expr -> structure (Tuple i (as_kind env)) o.
+    refine (
+match expr as expr in kappa i' o' return i = i' -> o = o' -> 
+wf_debrujin env expr -> structure (Tuple i (as_kind env)) o 
+with
+| DVar v => fun _ _ wf => _
+(* Instantiating a variable is done by 'cancell' to select the environment, and
+then indexing using lookup_morphism. *)
+| @DAbs _ x y z f => fun _ _ wf =>
+(* Kappa abstraction requires extending the environment then moving the 
+new environment variable in to place*)
+  let env' := ECons x env in
+  let f' := closure_conversion' _ _ _ env' (f n) (wf_debrujin_succ _ eq_refl wf) in
+  (* This line moves the first arrow argument into the right hand position,
+  which allows 'assoc' to move the argument to the front of the environment
+  f: x*y ~> o
 
-  Lemma lookup_upper_contra : forall o objs,
-    lookup_object (length objs) objs = Some o -> False.
-  Proof.
-    auto.
-  Qed.
+  f_kappa:    (x*y)*environment_variables ~> o
+  first swap: (y*x)*environment_variables ~> o
+  assoc:      y*(x*environment_variables) ~> o
+  f':         y*new_environment_variables ~> o
+  *)
+  _ (* first swap >>> assoc >>> f' *)
 
+  | DApp f e => fun _ _ wf =>
+  (* for application the Kind environment needs to be piped to the abstraction
+  'f' and applicant 'e'. since running 'closure_conversion' on each binder
+  removes the environment, we first need to copy the environment. *)
+  _
+  (* second (copy >>> first (uncancell
+  >>> closure_conversion' _ _ _ env e (proj2 _)))
+  >>> unassoc >>> first swap
+  >>> closure_conversion' _ _ _ env f (proj1 _) *)
+
+| DCompose e1 e2 => fun _ _ wf => _
+  (* second copy
+  >>> unassoc
+  >>> first (closure_conversion' env e2 (proj2 wf))
+  >>> closure_conversion' env e1 (proj1 wf) *)
+
+| DArr m => fun _ _ _ => _ (* cancelr >>> m *)
+end (eq_refl i) (eq_refl o)
+).
+- 
+  inversion wf.
+  assert (as_kind env ?? lookup_kind v (as_kind_list env) = structure (as_kind env) o).
+
+  rewrite H0.
+  rewrite e0.
+  reflexivity.
+
+  refine (First Drop >>> Cancell >>> _).
+  cbv [ConstructiveCat morphism].
+
+  rewrite <- H.
+  apply (extract_nth' (as_kind_list env) v (Kind_to_list_kind_id env)).
+
+- rewrite e, e0.
+  exact (first swap >>> assoc >>> f').
+
+- rewrite e0, e1.
+  destruct wf.
+  exact (
+    second (copy >>> first (uncancell
+    >>> closure_conversion' _ _ _ env e H0))
+    >>> unassoc >>> first swap
+    >>> closure_conversion' _ _ _ env f H
+  ).
+- rewrite e, e0.
+  destruct wf.
+  exact (
+  second copy
+  >>> unassoc
+  >>> first (closure_conversion' _ _ _ env e2 H0)
+  >>> closure_conversion' _ _ _ env e1 H
+).
+- rewrite e, e0.
+  exact (Second Drop >>> Cancelr >>> m).
+Defined.
+
+(****************************************************************************)
+(* Kappa term equivalence                                                   *)
+(****************************************************************************)
+
+Section Equivalence.
+  Inductive obj_tup :  Type := obj_pair : Kind -> Kind -> obj_tup.
+  Variables var1 var2 : Kind -> Kind -> Type.
+
+  Definition vars := existT (fun '(obj_pair x y) => (var1 x y * var2 x y)%type).
+  Definition ctxt := list { '(obj_pair x y) : obj_tup & (var1 x y * var2 x y)%type }.
+
+  Inductive kappa_equivalence:
+    forall i o, ctxt
+    -> @kappa var1 i o -> @kappa var2 i o
+    -> Prop :=
+  | Var_equiv : forall i o n1 n2 E,
+    In (vars (obj_pair i o) (pair n1 n2)) E
+    -> kappa_equivalence E (DVar n1) (DVar n2)
+
+  | Abs_equiv : forall o (f1: var1 unit o -> @kappa var1 unit o) f2 (E:ctxt),
+    (forall n1 n2, kappa_equivalence (vars (obj_pair unit o) (pair n1 n2) :: E) (f1 n1) (f2 n2))
+    -> kappa_equivalence E (DAbs f1) (DAbs f2)
+
+  | App_equiv : forall E x y z (f1 : @kappa var1 (x**y) z) f2 e1 e2,
+    kappa_equivalence E f1 f2
+    -> kappa_equivalence E e1 e2
+    -> kappa_equivalence E (DApp f1 e1) (DApp f2 e2)
+
+  | Compose_equiv : forall E x y z (f1 : @kappa var1 y z) f2 (g1: @kappa var1 x y) g2,
+    kappa_equivalence E f1 f2
+    -> kappa_equivalence E g1 g2
+    -> kappa_equivalence E (DCompose f1 g1) (DCompose f2 g2)
+
+  | Arr_equiv : forall x y E (m: morphism x y), kappa_equivalence E (DArr m) (DArr m) .
+End Equivalence.
+
+Axiom Kappa_equivalence : forall {i o} (expr: forall var, @kappa var i o) var1 var2,
+  kappa_equivalence nil (expr var1) (expr var2).
+
+Notation variable_pair i o n1 n2 := (vars natvar natvar (obj_pair i o) (pair n1 n2)).
+
+(* Evidence of variable pair equality *)
+Notation match_pairs xo xn yi yo yn1 yn2 :=
+  (variable_pair unit xo xn xn = variable_pair yi yo yn1 yn2).
+
+(* Evidence that if a given variable is in an environment we can lookup_kind the Kind at the index. *)
+Notation ok_variable_lookup := (fun env E =>
+  forall (i o : Kind) (n1 n2 : natvar i o),
+    In (vars natvar natvar (obj_pair i o) (pair n1 n2)) E
+    -> lookup_kind n1 (as_kind_list env) = Some o
+).
+
+(* Recovering a dependent value requires recovering the type equality first to prevent the
+value equality disappearing. *)
+Lemma recover_dependent_val: forall xo xn yi yo yn1 yn2,
+  match_pairs xo xn yi yo yn1 yn2 -> (xn = yn1 /\ xo = yo).
+Proof.
+  intros.
+  inversion H.
+  subst.
+  generalize (inj_pairT2 _ _ _ _ _ H).
+  intro.
+  inversion H0.
+  auto.
+Qed.
+
+Lemma apply_lookup : forall n (env: environment n) i o n1 n2 E,
+  In (variable_pair i o n1 n2) E
+  -> ok_variable_lookup env E
+  -> lookup_kind n1 (as_kind_list env) = Some o.
+Proof.
   Hint Extern 1 =>
     match goal with
-    | [H: lookup_object (length ?X) (?X) = Some _ |- _] => apply lookup_upper_contra in H; contradiction
-    | [H: lookup_object ?X [] = Some _ |- _] => apply lookup_lower_contra in H; contradiction
+    | [H1: In _ ?X, H2: ok_variable_lookup _ ?X |- _] => apply H2 in H1
     end : core.
+  auto.
+Qed.
 
-  (* Shorthand for passing evidence that a lookup is well formed *)
-  Notation ok_lookup := (
-    fun (n: nat) (env: list (bundle)) (o: bundle) => lookup_object n env = Some o
-  ).
+Lemma apply_extended_lookup: forall n env v1 v2 y i o E,
+  match_pairs y n i o v1 v2 \/ In (vars natvar natvar (obj_pair i o) (pair v1 v2)) E
+  -> ok_variable_lookup env E
+  -> lookup_kind v1 (as_kind_list (@ECons n y env)) = Some o.
+Proof.
+  Hint Extern 3 => eapply recover_dependent_val : core.
+  Hint Resolve split_lookup : core.
+  eauto 7.
+Qed.
 
-  (* Proof that looking up a morphism is the morphism from the environment to
-    * the object at the same index.
-    *)
-  Lemma ok_lookup_sets_lookup_morphism_ty : forall n o objs env_obj,
-    lookup_object n objs = Some o
-    -> lookup_morphism_ty n env_obj objs = structure env_obj o.
-  Proof.
-    induction objs; auto.
-  Qed.
+Hint Immediate apply_lookup : core.
+Hint Immediate apply_extended_lookup : core.
 
-  Hint Immediate ok_lookup_sets_lookup_morphism_ty : core.
+(* Apply the auto generated kappa_equivalence_ind induction scheme rather than
+calling induction directly as calling induction directly results in too
+specific hypotheses. *)
+Lemma kappa_wf
+  : forall i o E (expr1 expr2: @kappa natvar i o),
+  kappa_equivalence E expr1 expr2
+  -> forall n (env: environment n), ok_variable_lookup env E
+  -> wf_debrujin env expr1.
+Proof.
+  apply (kappa_equivalence_ind
+  (fun i o E (expr1 expr2 : @kappa natvar i o) =>
+    forall n (env: environment n),
+      ok_variable_lookup env E
+      -> wf_debrujin env expr1)
+      );eauto.
+Qed.
 
-  Lemma morphism_coerce:
-    forall (n:nat) env_obj o (objs: list (bundle)),
-    ok_lookup n objs o ->
-    lookup_morphism_ty n env_obj objs = structure env_obj o.
-  Proof.
-    auto.
-  Qed.
+Hint Resolve kappa_wf : core.
+Hint Resolve Kappa_equivalence : core.
 
-  Lemma environment_objects_length_is_n  (n: nat) (env: environment n):
-    length (as_object_list env) = n.
-  Proof.
-    induction env; auto.
-  Qed.
+Theorem Kappa_wf: forall {i o} (expr: forall var, @kappa var i o), @wf_debrujin _ _ 0 ENil (expr _).
+Proof.
+  eauto.
+Qed.
 
-  Hint Extern 4 =>
-    match goal with
-    | [H: context[length(as_object_list ?X)] |- _] => rewrite environment_objects_length_is_n in H
-    end : core.
-
-  Lemma split_lookup : forall n env v1 y o,
-    ((n = v1 /\ y = o) \/ lookup_object v1 (as_object_list env) = Some o)
-    -> lookup_object v1 (as_object_list (@ECons n y env)) = Some o.
-  Proof.
-    auto 6.
-  Qed.
-
-  Lemma unsplit_lookup : forall n env v1 y o,
-    lookup_object v1 (as_object_list (@ECons n y env)) = Some o
-    ->
-    ((n = v1 /\ y = o) \/ lookup_object v1 (as_object_list env) = Some o).
-  Proof.
-    auto 6.
-  Qed.
-
-  Lemma lookup_top_is_top_object: forall n m o o' env,
-    m = n
-    -> lookup_object m (as_object_list (@ECons n o env)) = Some o'
-    -> o = o'.
-  Proof.
-    auto.
-  Qed.
-
-  Lemma push_lookup : forall n env o o' x ,
-    x <> n ->
-    lookup_object x (as_object_list (@ECons n o' env)) = Some o ->
-    lookup_object x (as_object_list env) = Some o.
-  Proof.
-    Hint Extern 1 => lia : core.
-    auto.
-  Qed.
-
-  Fixpoint extract_nth n (env: environment n) o x
-    : (lookup_object x (as_object_list env) = Some o) -> structure (as_object env) o :=
-  match env return
-    (lookup_object x (as_object_list env) = Some o) -> structure (as_object env) o
-    with
-  | ENil => fun H => match lookup_lower_contra H with end
-  | @ECons n' o' env' => fun H =>
-    match eq_nat_dec x n' with
-    | left Heq =>
-      match lookup_top_is_top_object _ _ Heq H with
-      | eq_refl => Exl _ _
-      end
-    | right Hneq =>  Exr _ _ >>> extract_nth env' x (push_lookup _ _ Hneq H)
-    end
-  end.
-
-  Notation "i ?? x" := (
-      match x with
-      | None => Datatypes.unit
-      | Some o => structure i o
-      end) (no associativity, at level 70).
-
-  Fixpoint extract_nth' (env: list (bundle)) x : forall i (prefix: structure i (list_as_object env)), i ?? lookup_object x env :=
-  match env return
-    forall i (prefix: structure i (list_as_object env)), i ?? lookup_object x env
-    with
-  | [] => fun _ _ => tt
-  | o :: os => 
-    match eq_nat_dec x (length os) as Heq return forall i (prefix: structure i (list_as_object (o::os))), i ?? (if Heq
-      then Some o
-      else lookup_object x os
-    ) 
-    with
-    | left Heq => fun _ p => p >>> exl
-    | right Hneq => fun _ p => extract_nth' os x (p >>> exr)
-    end
-  end.
-
-  Lemma extractable : forall n env o,
-    lookup_object n env = Some o
-    -> forall i (prefix: structure i (list_as_object env)), i ?? lookup_object n env = structure i o.
-  Proof.
-    intros.
-    rewrite H.
-    reflexivity.
-  Defined.
-
-  (****************************************************************************)
-  (* Closure conversion via de Brujin indices form                            *)
-  (****************************************************************************)
-  (* In de Brujin indexing variables are nats *)
-
-  Definition natvar `{Category} : object -> object -> Type := fun _ _ => nat.
-
-  (* Reverse de Brujin indexing is well formed *)
-  Fixpoint wf_debrujin {i o}
-    (n: nat) (env: environment n)
-    (expr: kappa natvar i o) {struct expr}
-    : Prop :=
-  match expr with
-  | DVar x            => ok_lookup x (as_object_list env) o
-  | @DAbs _ x y z f => wf_debrujin (@ECons n x env) (f n)
-  | DApp e1 e2        => wf_debrujin env e1 /\ wf_debrujin env e2
-  | DCompose e1 e2    => wf_debrujin env e1 /\ wf_debrujin env e2
-  | DArr _            => True
-  end.
-
-  Lemma wf_debrujin_succ:
-    forall ix iy o
-    (n: nat) (env: environment n)
-    (expr: kappa natvar (Tuple2 ix iy) o)
-    f,
-    expr = DAbs f ->
-    @wf_debrujin (Tuple2 ix iy) o n env expr -> @wf_debrujin iy o (S n) (ECons ix env) (f n).
-  Proof.
-    auto.
-  Defined.
-
-
-  (* Perform closure conversion by passing an explicit environment. The higher
-  order PHOAS representation is converted to first order form with de Brujin
-  indexing as described by Adam Chlipala's Lambda Tamer project. As our source
-  language is a Kappa calculus and our target is a Generalized Arrow representation,
-  the environment and arguments are manipulated using Arrow combinators amongst
-  other differences.
-
-  This implementation is also currently missing logic to remove free variables
-  from the environment.
-  *)
-  Fixpoint closure_conversion' {i o}
-    (n: nat) (env: environment n)
-    (* (morphs: env_morphisms (as_object env) (as_object_list env)) *)
-    (expr: kappa natvar i o) {struct expr}
-    : wf_debrujin env expr -> structure (Tuple2 i (as_object env)) o.
-     refine (
-  match expr as expr in kappa _ i' o' return i = i' -> o = o' -> 
-  wf_debrujin env expr -> structure (Tuple2 i (as_object env)) o 
-  with
-  | DVar v => fun _ _ wf => _
-  (* Instantiating a variable is done by 'exr' to select the environment, and
-  then indexing using lookup_morphism. *)
-  | @DAbs _ x y z f => fun _ _ wf =>
-  (* Kappa abstraction requires extending the environment then moving the 
-  new environment variable in to place*)
-    let env' := ECons x env in
-    let f' := closure_conversion' _ _ _ env' (f n) (wf_debrujin_succ _ eq_refl wf) in
-    (* This line moves the first arrow argument into the right hand position,
-    which allows 'assoc' to move the argument to the front of the environment
-    f: x*y ~> o
-
-    f_kappa:    (x*y)*environment_variables ~> o
-    first swap: (y*x)*environment_variables ~> o
-    assoc:      y*(x*environment_variables) ~> o
-    f':         y*new_environment_variables ~> o
-    *)
-    _ (* first swap >>> assoc >>> f' *)
-
-    | DApp f e => fun _ _ wf =>
-    (* for application the object environment needs to be piped to the abstraction
-    'f' and applicant 'e'. since running 'closure_conversion' on each binder
-    removes the environment, we first need to copy the environment. *)
-    _
-    (* second (copy >>> first (uncancell
-    >>> closure_conversion' _ _ _ env e (proj2 _)))
-    >>> unassoc >>> first swap
-    >>> closure_conversion' _ _ _ env f (proj1 _) *)
-
-  | DCompose e1 e2 => fun _ _ wf => _
-    (* second copy
-    >>> unassoc
-    >>> first (closure_conversion' env e2 (proj2 wf))
-    >>> closure_conversion' env e1 (proj1 wf) *)
-
-  | DArr m => fun _ _ _ => _ (* exl >>> m *)
-  end (eq_refl i) (eq_refl o)
-  ).
-  - 
-    inversion wf.
-    assert (as_object env ?? lookup_object v (as_object_list env) = structure (as_object env) o).
-
-    rewrite H0.
-    rewrite e0.
-    reflexivity.
-
-    refine (Compose _ exr).
-
-    rewrite <- H.
-    apply (extract_nth' (as_object_list env) v (object_to_list_object_id env)).
-
-  - rewrite e, e0.
-    exact (first swap >>> assoc >>> f').
-
-  - rewrite e0, e1.
-    destruct wf.
-    exact (
-      second (copy >>> first (uncancell
-      >>> closure_conversion' _ _ _ env e H0))
-      >>> unassoc >>> first swap
-      >>> closure_conversion' _ _ _ env f H
-    ).
-  - rewrite e, e0.
-    destruct wf.
-    exact (
-    second copy
-    >>> unassoc
-    >>> first (closure_conversion' _ _ _ env e2 H0)
-    >>> closure_conversion' _ _ _ env e1 H
-  ).
-  - rewrite e, e0.
-    exact (exl >>> m).
-  Defined.
-
-  (****************************************************************************)
-  (* Kappa term equivalence                                                   *)
-  (****************************************************************************)
-
-  Section Equivalence.
-    Inductive obj_tup :  Type := obj_pair : object -> object -> obj_tup.
-    Variables var1 var2 : object -> object -> Type.
-
-    Definition vars := existT (fun '(obj_pair x y) => (var1 x y * var2 x y)%type).
-    Definition ctxt := list { '(obj_pair x y) : obj_tup & (var1 x y * var2 x y)%type }.
-
-    Inductive kappa_equivalence:
-      forall i o, ctxt
-      -> kappa var1 i o -> kappa var2 i o
-      -> Prop :=
-    | Var_equiv : forall i o n1 n2 E,
-      In (vars (obj_pair i o) (n1,n2)) E
-      -> kappa_equivalence E (DVar n1) (DVar n2)
-
-    | Abs_equiv : forall o (f1: var1 unit o -> kappa var1 unit o) f2 (E:ctxt),
-      (forall n1 n2, kappa_equivalence (vars (obj_pair unit o) (n1,n2) :: E) (f1 n1) (f2 n2))
-      -> kappa_equivalence E (DAbs f1) (DAbs f2)
-
-    | App_equiv : forall E x y z (f1 : kappa var1 (x**y) z) f2 e1 e2,
-      kappa_equivalence E f1 f2
-      -> kappa_equivalence E e1 e2
-      -> kappa_equivalence E (DApp f1 e1) (DApp f2 e2)
-
-    | Compose_equiv : forall E x y z (f1 : kappa var1 y z) f2 (g1: kappa var1 x y) g2,
-      kappa_equivalence E f1 f2
-      -> kappa_equivalence E g1 g2
-      -> kappa_equivalence E (DCompose f1 g1) (DCompose f2 g2)
-
-    | Arr_equiv : forall x y E (m: morphism x y), kappa_equivalence E (DArr m) (DArr m) .
-  End Equivalence.
-
-  Axiom Kappa_equivalence : forall {i o} (expr: forall var, kappa var i o) var1 var2,
-    kappa_equivalence nil (expr var1) (expr var2).
-
-  Notation variable_pair i o n1 n2 := (vars natvar natvar (obj_pair i o) (n1, n2)).
-
-  (* Evidence of variable pair equality *)
-  Notation match_pairs xo xn yi yo yn1 yn2 :=
-    (variable_pair unit xo xn xn = variable_pair yi yo yn1 yn2).
-
-  (* Evidence that if a given variable is in an environment we can lookup_object the object at the index. *)
-  Notation ok_variable_lookup := (fun env E =>
-    forall (i o : object) (n1 n2 : natvar i o),
-      In (vars natvar natvar (obj_pair i o) (n1, n2)) E
-      -> lookup_object n1 (as_object_list env) = Some o
-  ).
-
-  (* Recovering a dependent value requires recovering the type equality first to prevent the
-  value equality disappearing. *)
-  Lemma recover_dependent_val: forall xo xn yi yo yn1 yn2,
-    match_pairs xo xn yi yo yn1 yn2 -> (xn = yn1 /\ xo = yo).
-  Proof.
-    intros.
-    inversion H.
-    subst.
-    generalize (inj_pairT2 _ _ _ _ _ H).
-    intro.
-    inversion H0.
-    auto.
-  Qed.
-
-  Lemma apply_lookup : forall n (env: environment n) i o n1 n2 E,
-    In (variable_pair i o n1 n2) E
-    -> ok_variable_lookup env E
-    -> lookup_object n1 (as_object_list env) = Some o.
-  Proof.
-    Hint Extern 1 =>
-      match goal with
-      | [H1: In _ ?X, H2: ok_variable_lookup _ ?X |- _] => apply H2 in H1
-      end : core.
-    auto.
-  Qed.
-
-  Lemma apply_extended_lookup: forall n env v1 v2 y i o E,
-    match_pairs y n i o v1 v2 \/ In (vars natvar natvar (obj_pair i o) (v1, v2)) E
-    -> ok_variable_lookup env E
-    -> lookup_object v1 (as_object_list (@ECons n y env)) = Some o.
-  Proof.
-    Hint Extern 3 => eapply recover_dependent_val : core.
-    Hint Resolve split_lookup : core.
-    eauto 7.
-  Qed.
-
-  Hint Immediate apply_lookup : core.
-  Hint Immediate apply_extended_lookup : core.
-
-  (* Apply the auto generated kappa_equivalence_ind induction scheme rather than
-  calling induction directly as calling induction directly results in too
-  specific hypotheses. *)
-  Lemma kappa_wf
-    : forall i o E (expr1 expr2: kappa natvar i o),
-    kappa_equivalence E expr1 expr2
-    -> forall n (env: environment n), ok_variable_lookup env E
-    -> wf_debrujin env expr1.
-  Proof.
-    apply (kappa_equivalence_ind
-    (fun i o E (expr1 expr2 : kappa natvar i o) =>
-      forall n (env: environment n),
-        ok_variable_lookup env E
-        -> wf_debrujin env expr1)
-        );eauto.
-  Qed.
-
-  Hint Resolve kappa_wf : core.
-  Hint Resolve Kappa_equivalence : core.
-
-  Theorem Kappa_wf: forall {i o} (expr: forall var, kappa var i o), @wf_debrujin _ _ 0 ENil (expr _).
-  Proof.
-    eauto.
-  Qed.
-
-  Definition closure_conversion {i o} (expr: @Kappa i o) (wf: wf_debrujin ENil (expr _)): i ~> o
-    := uncancelr >>> closure_conversion' ENil (expr _) wf.
+Definition closure_conversion {i o} (expr: @Kappa i o) (wf: wf_debrujin ENil (expr _)): i ~> o
+  := uncancelr >>> closure_conversion' ENil (expr _) wf.
 
 Definition Closure_conversion {i o} (expr: @Kappa i o): i ~> o
   := closure_conversion expr (Kappa_wf expr).
