cava/cava/Cava/Arrow/Kappa/Kappa.v
@@ -1,80 +1,123 @@
 Require Import Cava.Arrow.Arrow.
 Require Import Cava.Arrow.Instances.Constructive.
 
-Section WithArrow.
+From Coq Require Import NArith.
 
-  Section Vars.
-    Variable var: object -> object -> Type.
+Section Vars.
+  Context {var: Kind -> Kind -> Type}.
 
-    Inductive kappa_sugared : object -> object -> Type :=
-    | Var: forall x y,    var x y -> kappa_sugared x y
-    | Abs: forall x y z,  (var unit x -> kappa_sugared y z) -> kappa_sugared (x ** y) z
-    | App: forall x y z,  kappa_sugared (x ** y) z -> kappa_sugared unit x -> kappa_sugared y z
-    | Com: forall x y z,  kappa_sugared y z -> kappa_sugared x y -> kappa_sugared x z
-    | Arr: forall x y,    morphism x y -> kappa_sugared x y
-    | Let: forall x y z,  kappa_sugared unit x -> (var unit x -> kappa_sugared y z) -> kappa_sugared y z.
+  (* `kappa_sugared` includes constructors for 
+    - Kappa Calculus, 
+    - the Cava methods, 
+    - lifting any morphism from the Constructive arrow instance, 
+    - and miscellaneous methods 
 
-    Inductive kappa : object -> object -> Type :=
-    | DVar : forall x y,   var x y -> kappa x y
-    | DAbs : forall x y z, (var unit x -> kappa y z) -> kappa (x**y) z
-    | DApp : forall x y z, kappa (x**y) z -> kappa unit x -> kappa y z
-    | DCompose : forall x y z, kappa y z -> kappa x y -> kappa x z
-    | DArr : forall x y,   morphism x y -> kappa x y.
-  End Vars.
+    The kappa calculus and LiftMorphism constructors are the only 5 
+    "primitive"/required constructors, the rest are a to help syntax 
+    or type inference and desugar simply to combinations of the others.
+    *)
+  Inductive kappa_sugared : Kind -> Kind -> Type :=
+    (* Kappa Calculus *)
+    | Var: forall {x y},    var x y -> kappa_sugared x y
+    | Abs: forall {x y z},  (var Unit x -> kappa_sugared y z) -> kappa_sugared << x, y >> z
+    | App: forall {x y z},  kappa_sugared << x, y >> z -> kappa_sugared Unit x -> kappa_sugared y z
+    | Com: forall {x y z},  kappa_sugared y z -> kappa_sugared x y -> kappa_sugared x z
 
-  Arguments Var [var x y].
-  Arguments Abs [var x y z].
-  Arguments App [var x y z].
-  Arguments Com [var x y z].
-  Arguments Arr [var x y].
-  Arguments Let [var x y z].
+    (* Lift any morphism from ConstructiveCat *)
+    | LiftMorphism: forall {x y},    morphism x y -> kappa_sugared x y
 
-  Arguments DVar [var x y].
-  Arguments DAbs [var x y z].
-  Arguments DApp [var x y z].
-  Arguments DCompose [var x y z].
-  Arguments DArr [var x y].
+    (* Helper syntax *)
+    | Let: forall {x y z},  kappa_sugared Unit x -> (var Unit x -> kappa_sugared y z) -> kappa_sugared y z
+    | TupleLeft: forall {x y}, kappa_sugared << << x, y >>, Unit >> x
+    | TupleRight: forall {x y}, kappa_sugared << << x, y >>, Unit >> y
+    | MakeTuple: forall {x y}, kappa_sugared << x, y, Unit >> << x, y >>
+      
+    (* Cava routines *)
+    | Constant: bool -> kappa_sugared Unit Bit
+    | ConstantVec: forall {n}, N -> kappa_sugared Unit (Vector n Bit)
+    | Not: kappa_sugared << Bit, Unit >> Bit
+    | And: kappa_sugared << Bit, Bit, Unit >> Bit
+    | Nand: kappa_sugared << Bit, Bit, Unit >> Bit
+    | Or:   kappa_sugared << Bit, Bit, Unit >> Bit
+    | Nor:  kappa_sugared << Bit, Bit, Unit >> Bit
+    | Xor:  kappa_sugared << Bit, Bit, Unit >> Bit
+    | Xnor: kappa_sugared << Bit, Bit, Unit >> Bit
+    | Buf:  kappa_sugared << Bit, Unit >>      Bit
+    | Delay: forall {o}, kappa_sugared << o, Unit >> o
+    | Xorcy: kappa_sugared << Bit, Bit, Unit >> Bit
+    | Muxcy: kappa_sugared << Bit, Tuple Bit Bit, Unit >> Bit
+    | UnsignedAdd: forall a b c, kappa_sugared << Vector a Bit, Vector b Bit, Unit >> (Vector c Bit)
+    (* TODO: enable lut *)
+    (*| Lut n: (bool^^n --> bool) -> bitvec (N.of_nat n) ~> bit;*)
+    | IndexVec: forall n {o}, kappa_sugared << Vector n o, Vector (N.log2_up n) Bit, Unit >> o
+    | ToVec: forall {o}, kappa_sugared << o, Unit >> (Vector 1 o)
+    | Concat: forall n {o}, kappa_sugared << Vector n o, o, Unit >> (Vector (n+1) o).
 
-  Definition Kappa_sugared i o := forall var, @kappa_sugared var i o.
-  Definition Kappa i o := forall var, @kappa var i o.
+  Bind Scope constructive_scope with kappa_sugared.
+  Delimit Scope constructive_scope with kappa_sugared.
 
-  (* desugars let bindings *)
-  Fixpoint desugar {var i o} (e: kappa_sugared var i o) : kappa var i o :=
+  (* Everything not manipulation a variable is mapped to its arrow representation via DArr.
+  So after desugaring the type is much simpler *)
+  Inductive kappa : Kind -> Kind -> Type :=
+    | DVar : forall {x y},   var x y -> kappa x y
+    | DAbs : forall {x y z}, (var Unit x -> kappa y z) -> kappa << x, y >> z
+    | DApp : forall {x y z}, kappa << x, y >> z -> kappa Unit x -> kappa y z
+    | DCompose : forall {x y z}, kappa y z -> kappa x y -> kappa x z
+    | DArr : forall {x y},   morphism x y -> kappa x y.
+End Vars.
+
+Definition Kappa_sugared i o := forall var, @kappa_sugared var i o.
+Definition Kappa i o := forall var, @kappa var i o.
+
+Definition kappa_app {var o} i (m: remove_rightmost_unit i ~> o) : @kappa var i o := DCompose (DArr m) (DArr (remove_rightmost_tt _)).
+
+Definition remove_second {x y}: structure << x, y >> x := (Compose Cancelr (Second Drop)).
+Definition remove_first {x y}: structure << x, y >> y := (Compose Cancell (First Drop)).
+
+Definition tuple_left {var x y}: @kappa var << <<x, y>> , Unit>> x
+  := DArr (Compose remove_second Cancelr).
+Definition tuple_right {var x y}: @kappa var << <<x, y>>, Unit>> y
+  := DArr (Compose remove_first Cancelr).
+
+Fixpoint desugar {var i o} (e: @kappa_sugared var i o) : @kappa var i o :=
   match e with
   | Var x => DVar x
   | Abs f => DAbs (fun x => desugar (f x))
   | App e1 e2 => DApp (desugar e1) (desugar e2)
   | Com f g => DCompose (desugar f) (desugar g)
-  | Arr m => DArr m
   | Let x f => DApp (DAbs (fun x => desugar (f x))) (desugar x)
+  | LiftMorphism m => DArr m
+
+  | TupleLeft  => tuple_left
+  | TupleRight  => tuple_right
+
+  | MakeTuple => DArr (Second Cancelr)
+
+  | Not  => kappa_app << Bit, Unit >> not_gate
+  | And  => kappa_app << Bit, Bit, Unit >> and_gate
+  | Nand => kappa_app << Bit, Bit, Unit >> nand_gate
+  | Or   => kappa_app << Bit, Bit, Unit >> or_gate
+  | Nor  => kappa_app << Bit, Bit, Unit >> nor_gate
+  | Xor  => kappa_app << Bit, Bit, Unit >> xor_gate
+  | Xnor => kappa_app << Bit, Bit, Unit >> xnor_gate
+  | Buf  => kappa_app << Bit, Unit >> buf_gate
+
+  | Delay  => DArr (Compose delay_gate Cancelr)
+
+  | Xorcy  => kappa_app << Bit, Bit, Unit >> xorcy 
+  | Muxcy  => kappa_app << Bit, Tuple Bit Bit, Unit >> muxcy 
+  | UnsignedAdd a b c => kappa_app << Vector a Bit, Vector b Bit, Unit >> (unsigned_add a b c)
+
+  | Constant b => DArr (constant b)
+  | ConstantVec v => DArr (constant_bitvec _ v)
+
+  | IndexVec n => kappa_app << Vector n _, Vector (N.log2_up n) Bit, Unit >> (index_vec n _)
+  | ToVec => kappa_app << _, Unit >> (to_vec _)
+  | Concat n => kappa_app << Vector n _, _, Unit >> (concat n _)
   end.
 
-  Definition Desugar {i o} (e: Kappa_sugared i o) : Kappa i o := fun var => desugar (e var).
+Definition tupleHelper {var X Y} x y :=  App (App (@MakeTuple var X Y) x) y.
+Definition Desugar {i o} (e: Kappa_sugared i o) : Kappa i o := fun var => desugar (e var).
 
-  (* reproject into unsugared into kappa *)
-  Fixpoint kappa_project {var i o} (e: kappa var i o) : kappa_sugared var i o :=
-  match e with
-  | DVar x => Var x
-  | DAbs f => Abs (fun x => kappa_project (f x))
-  | DApp e1 e2 => App (kappa_project e1) (kappa_project e2)
-  | DCompose f g => Com (kappa_project f) (kappa_project g)
-  | DArr m => Arr m
-  end.
-
-  Hint Resolve Desugar : core.
-  Hint Resolve desugar : core.
-
-End WithArrow.
-
-Arguments Var [var x y].
-Arguments Abs [var x y z].
-Arguments App [var x y z].
-Arguments Com [var x y z].
-Arguments Arr [var x y].
-Arguments Let [var x y z].
-
-Arguments DVar [var x y].
-Arguments DAbs [var x y z].
-Arguments DApp [var x y z].
-Arguments DCompose [var x y z].
-Arguments DArr [var x y].
+Hint Resolve Desugar : core.
+Hint Resolve desugar : core.
