cava/arrow-examples/Concatenative/Nand.v
@@ -1,6 +1,0 @@
-Require Import Cava.Arrow.Arrow.
-
-(* Implement a NAND circuit by composing an AND gate and INV gate. *)
-Definition nand
-  `{Cava}
-  := second uncancelr >>> and_gate >>> uncancelr >>> not_gate.
